pulse/lib/steel/pulse/Pulse.Typing.Metatheory.fsti
@@ -80,115 +80,248 @@ let st_typing_equiv_pre (#g:env) (#t:st_term) (#c:comp_st) (d:st_typing g t c)
 
 ///// Substitution lemma /////
 
+module Psubst = Pulse.Prover.Substs
+
 module L = FStar.List.Tot
 let map_opt (#a #b:Type) (f:a -> b) (x:option a) : option b =
   match x with
   | None -> None
   | Some x -> Some (f x)
 
-let subst_flip (ss:subst) (t:term) = subst_term t ss
+let subst_flip ss t = subst_term t ss
 
 let subst_env (en:env) (ss:subst)
   : en':env { fstar_env en == fstar_env en' /\
               dom en == dom en' /\
-              (forall (x:var). lookup en' x ==
+              (forall (x:var).{:pattern lookup en' x}
+                               lookup en' x ==
                                map_opt (subst_flip ss) (lookup en x)) }
   = admit ()
 
-type nt_subst = s:subst {
-  forall (elt:subst_elt). List.Tot.memP elt s ==> NT? elt
-}
+module RT = FStar.Reflection.Typing
+let subst_env_mk_env (f:RT.fstar_top_env) (ss:subst)
+  : Lemma (subst_env (mk_env f) ss == mk_env f)
+          [SMTPat (subst_env (mk_env f) ss)] = admit ()
+
+let well_typed_ss (#g:env) (g':env) (ss:Psubst.t g) =
+
+  forall (x:var).{:pattern Set.mem x (Psubst.dom ss) }
+  Set.mem x (Psubst.dom ss) ==> (x `Set.mem` dom g' /\
+                                (let Some t = lookup g' x in
+                                 tot_typing g (Psubst.lookup ss x)
+                                              (Psubst.subst_term ss t)))
 
 let pairwise_disjoint (g g' g'':env) =
   disjoint g g' /\ disjoint g' g'' /\ disjoint g g''
 
-let rec lookup_nt_subst (ss:nt_subst) (x:var) : option term =
-  match ss with
-  | [] -> None
-  | (NT y t)::ss -> if x = y then Some t else lookup_nt_subst ss x
+let singleton_env (f:_) (x:var) (t:typ) = push_binding (mk_env f) x t
 
-let well_typed_ss (g:env) (g':env) (ss:nt_subst) =
+let nt (x:var) (t:term) = [ NT x t ]
 
-  forall (elt:subst_elt).
-  L.memP elt ss ==> (let NT x e = elt in
-                     x `Set.mem` dom g' /\
-                     (let Some t = lookup g' x in
-                      tot_typing g e (subst_term t ss)))
-
-let ss_covers_g' (ss:nt_subst) (g':env) =
-  forall (x:var). x `Set.mem` dom g' ==> Some? (lookup_nt_subst ss x)
-
-let tot_typing_subst (g:env) (g':env) (g'':env { pairwise_disjoint g g' g'' })
-  (#e1:term) (#t1:typ)
-  (e1_typing:tot_typing (push_env g (push_env g' g'')) e1 t1)
-  (ss:nt_subst { well_typed_ss g g' ss /\ ss_covers_g' ss g' })
-  : tot_typing (push_env g (subst_env g'' ss)) (subst_term e1 ss) (subst_term t1 ss) = admit ()
-  
-let rec st_typing_subst (g:env) (g':env) (g'':env { pairwise_disjoint g g' g'' })
+let st_typing_subst
+  (g:env) (x:var) (t:typ) (g':env { pairwise_disjoint g (singleton_env (fstar_env g) x t) g' })
+  (#e:term)
+  (e_typing:tot_typing g e t)
   (#e1:st_term) (#c1:comp_st)
-  (e1_typing:st_typing (push_env g (push_env g' g'')) e1 c1)
-  (ss:nt_subst { well_typed_ss g g' ss /\ ss_covers_g' ss g' })
-  : st_typing (push_env g (subst_env g'' ss)) (subst_st_term e1 ss) (subst_comp c1 ss) =
+  (e1_typing:st_typing (push_env g (push_env (singleton_env (fstar_env g) x t) g')) e1 c1)
 
-  match e1_typing with
-  | T_Abs _ x q b u body c b_ty_typing body_typing ->
-    let b_ty_typing
-      : tot_typing (push_env g g'')
-                   (subst_term b.binder_ty ss)
-                   (tm_type u) = tot_typing_subst g g' g'' b_ty_typing ss in
-    
-    let g1 : env = push_binding (push_env g (push_env g' g'')) x (subst_term b.binder_ty ss) in
-    let g2 : env = push_env g (push_env g' (push_binding g'' x (subst_term b.binder_ty ss))) in
-    assume (bindings g1 == bindings g2);
+  : st_typing (push_env g (subst_env g' (nt x t)))
+              (subst_st_term e1 (nt x e))
+              (subst_comp c1 (nt x e)) =
   
-    let body_typing
-      : st_typing g1 (open_st_term_nv (subst_st_term body ss) (b.binder_ppname, x)) (subst_comp c ss)
-      = st_typing_subst g g' (push_binding g'' x (subst_term b.binder_ty ss)) body_typing ss in
-
-    T_Abs _ x q (subst_binder b ss) u (subst_st_term body ss) (subst_comp c ss)
-          b_ty_typing body_typing
-
-  | T_STApp _ head ty q res arg head_typing arg_typing ->
-    assume (subst_term (tm_arrow (as_binder ty) q res) ss ==
-            tm_arrow (as_binder (subst_term ty ss)) q (subst_comp res ss));
-    assume (subst_comp (open_comp_with res arg) ss ==
-            open_comp_with (subst_comp res ss) (subst_term arg ss));
-    T_STApp _ (subst_term head ss) (subst_term ty ss) q
-              (subst_comp res ss) (subst_term arg ss)
-              (tot_typing_subst g g' g'' head_typing ss)
-              (tot_typing_subst g g' g'' arg_typing ss)
-
-  | _ -> admit ()
-
-let veq_subst (g:env) (g':env) (g'':env { pairwise_disjoint g g' g'' })
-  (#p1 #p2:vprop)
-  (veq:vprop_equiv (push_env g (push_env g' g'')) p1 p2)
-  (ss:nt_subst { well_typed_ss g g' ss /\ ss_covers_g' ss g' })
-  : vprop_equiv (push_env g (subst_env g'' ss)) (subst_term p1 ss) (subst_term p2 ss) = admit ()
-
-
-let st_subst_partial (g:env) (g':env) (g'':env { pairwise_disjoint g g' g'' })
-  (#e1:st_term) (#c1:comp_st)
-  (e1_typing:st_typing (push_env g (push_env g' g'')) e1 c1)
-  (ss:nt_subst { well_typed_ss g g' ss })
-  : st_typing (push_env g (push_env g' (subst_env g'' ss))) (subst_st_term e1 ss) (subst_comp c1 ss) =
   admit ()
 
-let veq_subst_partial (g:env) (g':env) (g'':env { pairwise_disjoint g g' g'' })
-  (#p1 #p2:vprop)
-  (veq:vprop_equiv (push_env g (push_env g' g'')) p1 p2)
-  (ss:nt_subst { well_typed_ss g g' ss })
-  : vprop_equiv (push_env g (push_env g' (subst_env g'' ss))) (subst_term p1 ss) (subst_term p2 ss) = admit ()
+let psubst_env (#g0:_) (g:env) (ss:Psubst.t g0) =
+  subst_env g (Psubst.as_subst ss)
 
-val ss_extends (s1 s2:nt_subst) : bool
+// different from extends, g1 may have dropped bindings from anywhere, not just the end
+let subenv (g1 g2:env) =
+  fstar_env g1 == fstar_env g2 /\
+  (forall (x:var).{:pattern Set.mem x (dom g1)}
+                  Set.mem x (dom g1) ==>
+                  (Set.mem x (dom g2) /\
+                   lookup g1 x == lookup g2 x))
 
-val ss_extends_subst (g:env) (g':env) (g'':env { g'' `env_extends` g' /\
-                                                 disjoint g g' /\
-                                                 disjoint g g'' })
-  (s':nt_subst)
-  (s'':nt_subst { s'' `ss_extends` s' /\
-                  well_typed_ss g g' s' /\
-                  well_typed_ss g g'' s'' })
-  (t:term { freevars (subst_term t s') `Set.subset` dom g })
-  : Lemma (subst_term t s' == subst_term t s'')
+let rec filter_ss (#g0:env) (g:env) (ss:Psubst.t g0)
+  : Tot (g':env { subenv g' g /\ Set.disjoint (dom g') (Psubst.dom ss) })
+        (decreases bindings g) =
+
+  match bindings g with
+  | [] -> mk_env (fstar_env g)
+  | _ ->
+    let ( x, t, g ) = remove_latest_binding g in
+    let g = filter_ss g ss in
+    if Set.mem x (Psubst.dom ss) then g
+    else push_binding g x t
+
+let coerce_eq (#a #b:Type) (x:a) (_:squash (a == b)) : y:b{y === x} = x
+
+// #push-options "--z3rlimit_factor 10 --fuel 2 --ifuel 2"
+// #push-options "--z3rlimit_factor 4"
+// #push-options "--z3rlimit_factor 4 --fuel 1 --ifuel 1"
+#push-options "--z3rlimit 50 --fuel 2 --ifuel 1"
+let rec apply_partial_psubs (g0:env) (t:st_term) (c:comp_st)
+  (uvs:env { disjoint uvs g0 })
+  (ss:Psubst.t g0 { well_typed_ss uvs ss })
+
+  (ss_consumed:Psubst.t g0)
+  (ss_remaining:Psubst.t g0 { Set.disjoint (Psubst.dom ss_consumed) (Psubst.dom ss_remaining) /\
+                              ss == Psubst.push ss_consumed ss_remaining })
+
+  (uvs_seen:env { Set.subset (Psubst.dom ss_consumed) (dom uvs_seen) })
+  (uvs_remaining:env { disjoint uvs_seen uvs_remaining /\
+                       uvs == push_env uvs_seen uvs_remaining /\
+                       Psubst.dom ss_remaining `Set.subset` dom uvs_remaining })
+
+  (uvs_unresolved:env { uvs_unresolved == filter_ss uvs_seen ss_consumed })
+
+  (t_typing:
+     st_typing (push_env g0 (psubst_env (push_env uvs_unresolved uvs_remaining) ss_consumed))
+               (Psubst.subst_st_term ss_consumed t)
+               (Psubst.subst_comp ss_consumed c))
+  
+  : Tot (uvs_unresolved:env { uvs_unresolved == filter_ss uvs ss } &
+         st_typing (push_env g0 (psubst_env uvs_unresolved ss))
+                   (Psubst.subst_st_term ss t)
+                   (Psubst.subst_comp ss c))
+        (decreases List.Tot.length (bindings uvs_remaining)) =
+  
+  match bindings uvs_remaining with
+  | [] ->
+    assert (equal uvs_remaining (mk_env (fstar_env g0)));
+    assert (Psubst.equal ss_remaining (Psubst.empty g0));
+    assert (Psubst.equal (Psubst.push ss_consumed (Psubst.empty g0)) ss_consumed);
+    assert (Psubst.equal ss_consumed ss);
+    assert (equal uvs_seen uvs);
+    assert (equal (push_env uvs_unresolved uvs_remaining) uvs_unresolved);
+    (| uvs_unresolved, t_typing |)
+  | _ ->
+    let (x, ty, uvs_remaining_new) = remove_binding uvs_remaining in
+    let g_x_t = push_binding (mk_env (fstar_env uvs_remaining)) x ty in
+    // assert (uvs_remaining == push_env g_x_t uvs_remaining_new);
+      
+    let uvs_seen_new = push_binding uvs_seen x ty in
+      
+    push_env_assoc uvs_seen g_x_t uvs_remaining_new;
+    assert (equal uvs (push_env uvs_seen_new uvs_remaining_new));
+    assert (disjoint uvs_seen_new uvs_remaining_new);
+    assume (List.Tot.length (bindings uvs_remaining_new) <
+            List.Tot.length (bindings uvs_remaining));
+
+
+    if not (x `Set.mem` Psubst.dom ss_remaining)
+    then begin
+      let uvs_unresolved_new = push_binding uvs_unresolved x ty in
+
+      push_env_assoc uvs_unresolved g_x_t uvs_remaining_new;
+      assert (equal (push_env uvs_unresolved uvs_remaining)
+                    (push_env uvs_unresolved_new uvs_remaining_new));
+
+      // assert (~ (x `Set.mem` Psubst.dom (ss_consumed)));
+      // (assert (let x', ty', g' = remove_latest_binding uvs_seen_new in
+      //          x == x' /\ ty == ty' /\ equal g' uvs_seen));
+      // This should be easy, with the commented assert above,
+      //   but my guess is some z3 loop
+      assume (equal uvs_unresolved_new (filter_ss uvs_seen_new ss_consumed));
+
+      let t_typing:
+        st_typing (push_env g0 (psubst_env (push_env uvs_unresolved_new uvs_remaining_new) ss_consumed))
+                  (Psubst.subst_st_term ss_consumed t)
+                  (Psubst.subst_comp ss_consumed c) =
+        coerce_eq t_typing () in
+
+      apply_partial_psubs g0 t c uvs ss ss_consumed ss_remaining
+        uvs_seen_new uvs_remaining_new uvs_unresolved_new t_typing
+    end
+    else admit ()
+    // let (x, ty, uvs_pending_suffix_tl ) = remove_binding uvs_pending_suffix in
+    // if not (x `Set.mem` Psubst.dom ss_remaining)
+    // then begin
+    //   push_env_assoc uvs_pending_prefix
+    //                  (push_binding (mk_env (fstar_env uvs_pending_suffix)) x ty)
+    //                  uvs_pending_suffix_tl;
+    //   assert (equal (push_env uvs_pending_prefix uvs_pending_suffix)
+    //                 (push_env (push_env uvs_pending_prefix
+    //                                     (push_binding (mk_env (fstar_env uvs_pending_suffix)) x ty))
+    //                           uvs_pending_suffix_tl));
+    //   admit ()
+    // end
+    // else admit ()
+
+
+// let ss_covers_g' (ss:nt_subst) (g':env) =
+//   forall (x:var). x `Set.mem` dom g' ==> Some? (lookup_nt_subst ss x)
+
+// let tot_typing_subst (g:env) (g':env) (g'':env { pairwise_disjoint g g' g'' })
+//   (#e1:term) (#t1:typ)
+//   (e1_typing:tot_typing (push_env g (push_env g' g'')) e1 t1)
+//   (ss:nt_subst { well_typed_ss g g' ss /\ ss_covers_g' ss g' })
+//   : tot_typing (push_env g (subst_env g'' ss)) (subst_term e1 ss) (subst_term t1 ss) = admit ()
+  
+// let rec st_typing_subst (g:env) (g':env) (g'':env { pairwise_disjoint g g' g'' })
+//   (#e1:st_term) (#c1:comp_st)
+//   (e1_typing:st_typing (push_env g (push_env g' g'')) e1 c1)
+//   (ss:nt_subst { well_typed_ss g g' ss /\ ss_covers_g' ss g' })
+//   : st_typing (push_env g (subst_env g'' ss)) (subst_st_term e1 ss) (subst_comp c1 ss) =
+
+//   match e1_typing with
+//   | T_Abs _ x q b u body c b_ty_typing body_typing ->
+//     let b_ty_typing
+//       : tot_typing (push_env g g'')
+//                    (subst_term b.binder_ty ss)
+//                    (tm_type u) = tot_typing_subst g g' g'' b_ty_typing ss in
+    
+//     let g1 : env = push_binding (push_env g (push_env g' g'')) x (subst_term b.binder_ty ss) in
+//     let g2 : env = push_env g (push_env g' (push_binding g'' x (subst_term b.binder_ty ss))) in
+//     assume (bindings g1 == bindings g2);
+  
+//     let body_typing
+//       : st_typing g1 (open_st_term_nv (subst_st_term body ss) (b.binder_ppname, x)) (subst_comp c ss)
+//       = st_typing_subst g g' (push_binding g'' x (subst_term b.binder_ty ss)) body_typing ss in
+
+//     T_Abs _ x q (subst_binder b ss) u (subst_st_term body ss) (subst_comp c ss)
+//           b_ty_typing body_typing
+
+//   | T_STApp _ head ty q res arg head_typing arg_typing ->
+//     assume (subst_term (tm_arrow (as_binder ty) q res) ss ==
+//             tm_arrow (as_binder (subst_term ty ss)) q (subst_comp res ss));
+//     assume (subst_comp (open_comp_with res arg) ss ==
+//             open_comp_with (subst_comp res ss) (subst_term arg ss));
+//     T_STApp _ (subst_term head ss) (subst_term ty ss) q
+//               (subst_comp res ss) (subst_term arg ss)
+//               (tot_typing_subst g g' g'' head_typing ss)
+//               (tot_typing_subst g g' g'' arg_typing ss)
+
+//   | _ -> admit ()
+
+// let veq_subst (g:env) (g':env) (g'':env { pairwise_disjoint g g' g'' })
+//   (#p1 #p2:vprop)
+//   (veq:vprop_equiv (push_env g (push_env g' g'')) p1 p2)
+//   (ss:nt_subst { well_typed_ss g g' ss /\ ss_covers_g' ss g' })
+//   : vprop_equiv (push_env g (subst_env g'' ss)) (subst_term p1 ss) (subst_term p2 ss) = admit ()
+
+// let st_subst_partial (g:env) (g':env) (g'':env { pairwise_disjoint g g' g'' })
+//   (#e1:st_term) (#c1:comp_st)
+//   (e1_typing:st_typing (push_env g (push_env g' g'')) e1 c1)
+//   (ss:nt_subst { well_typed_ss g g' ss })
+//   : st_typing (push_env g (push_env g' (subst_env g'' ss))) (subst_st_term e1 ss) (subst_comp c1 ss) =
+//   admit ()
+
+// let veq_subst_partial (g:env) (g':env) (g'':env { pairwise_disjoint g g' g'' })
+//   (#p1 #p2:vprop)
+//   (veq:vprop_equiv (push_env g (push_env g' g'')) p1 p2)
+//   (ss:nt_subst { well_typed_ss g g' ss })
+//   : vprop_equiv (push_env g (push_env g' (subst_env g'' ss))) (subst_term p1 ss) (subst_term p2 ss) = admit ()
+
+// val ss_extends (s1 s2:nt_subst) : bool
+
+// val ss_extends_subst (g:env) (g':env) (g'':env { g'' `env_extends` g' /\
+//                                                  disjoint g g' /\
+//                                                  disjoint g g'' })
+//   (s':nt_subst)
+//   (s'':nt_subst { s'' `ss_extends` s' /\
+//                   well_typed_ss g g' s' /\
+//                   well_typed_ss g g'' s'' })
+//   (t:term { freevars (subst_term t s') `Set.subset` dom g })
+//   : Lemma (subst_term t s' == subst_term t s'')
 
