pulse/lib/steel/pulse/Pulse.Prover.Substs.fst
@@ -1,0 +1,190 @@
+module Pulse.Prover.Substs
+
+open Pulse.Syntax
+
+module L = FStar.List.Tot
+
+module R = FStar.Reflection
+module RT = FStar.Reflection.Typing
+
+open FStar.List.Tot
+
+type bmap = m:Map.t var typ {
+  forall (x:var). (~ (Map.contains m x)) ==> (Map.sel m x == Tm_Unknown)
+}
+
+let remove_binding ((x, _):var & typ) (m:bmap) : bmap =
+  Map.restrict (Set.complement (Set.singleton x)) (Map.upd m x Tm_Unknown)
+
+let related (bs:list (var & typ)) (m:Map.t var typ) =
+  (forall (b:var & typ).
+          L.memP b bs ==> (Map.contains m (fst b) /\
+                           Map.sel m (fst b) == snd b)) /\
+  
+  (forall (x:var). Map.contains m x ==> (List.Tot.memP (x, Map.sel m x) bs))
+
+noeq
+type env = {
+  f : RT.fstar_top_env;
+  bs : list (var & typ);
+  m : m:bmap { related bs m };
+  ctxt: Pulse.RuntimeUtils.context
+}
+
+let fstar_env g = g.f
+
+let bindings g = g.bs
+
+let as_map g = g.m
+
+let bindings_as_map _ = ()
+
+let empty_bmap : bmap = Map.const_on Set.empty Tm_Unknown
+
+let equal_elim g1 g2 = assert (Map.equal g1.m g2.m)
+
+let default_context : Pulse.RuntimeUtils.context = FStar.Sealed.seal []
+
+let mk_env (f:RT.fstar_top_env) : env = { f; bs = []; m = empty_bmap; ctxt = default_context }
+
+let mk_env_bs _ = ()
+
+let push_binding g x t =
+  { g with bs = (x, t)::g.bs; m = Map.upd g.m x t }
+
+let push_binding_bs _ _ _ = ()
+
+let push_binding_as_map _ _ _ = ()
+
+let rec max (bs:list (var & typ)) (current:var)
+  : v:var { current <= v /\ (forall (b:var & typ). List.Tot.memP b bs ==> fst b <= v) } =
+  match bs with
+  | [] -> current
+  | (x, t)::rest ->
+    let current = if x < current then current else x in
+    max rest current
+
+let fresh g =
+  match g.bs with
+  | [] -> 1
+  | (x, _)::bs_rest ->
+    let max = max bs_rest x in
+    max + 1
+
+//
+// TODO: Move to ulib
+//
+let rec append_memP (#a:Type) (l1 l2:list a) (x:a)
+  : Lemma (L.memP x (l1 @ l2) <==> (L.memP x l1 \/ L.memP x l2))
+          [SMTPat (L.memP x (l1 @ l2))] =
+  match l1 with
+  | [] -> ()
+  | _::tl -> append_memP tl l2 x
+
+let push_env (g1:env) (g2:env { disjoint g1 g2 }) : env =
+  { f = g1.f; bs = g2.bs @ g1.bs; m = Map.concat g2.m g1.m; ctxt = g1.ctxt }
+
+let push_env_fstar_env _ _ = ()
+
+let push_env_bindings _ _ = ()
+
+let push_env_as_map _ _ = ()
+
+let push_env_assoc g1 g2 g3 =
+  L.append_assoc g3.bs g2.bs g1.bs;
+  assert (equal (push_env g1 (push_env g2 g3)) (push_env (push_env g1 g2) g3))
+
+let intro_env_extends (g1 g2 g3:env)
+  : Lemma (requires extends_with g1 g2 g3)
+          (ensures g1 `env_extends` g2) = ()
+
+let elim_env_extends (g1:env) (g2:env { g1 `env_extends` g2 })
+  : GTot (g3:env { extends_with g1 g2 g3 }) =
+  FStar.IndefiniteDescription.indefinite_description_ghost
+    env (fun g3 -> extends_with g1 g2 g3)
+
+let env_extends_refl (g:env) : Lemma (g `env_extends` g) =
+  assert (equal g (push_env g (mk_env g.f)));
+  intro_env_extends g g (mk_env g.f)
+
+let env_extends_trans (g1 g2 g3:env)
+  : Lemma (requires g1 `env_extends` g2 /\ g2 `env_extends` g3)
+          (ensures g1 `env_extends` g3) =
+  let g12 = elim_env_extends g1 g2 in
+  let g23 = elim_env_extends g2 g3 in
+  L.append_assoc g12.bs g23.bs g3.bs;
+  assert (equal g1 (push_env g3 (push_env g23 g12)));
+  intro_env_extends g1 g3 (push_env g23 g12)
+
+let env_extends_push (g:env) (x:var { ~ (Set.mem x (dom g)) }) (t:typ)
+  : Lemma (push_binding g x t `env_extends` g) =
+  assert (equal (push_binding g x t) (push_env g (push_binding (mk_env g.f) x t)));
+  intro_env_extends (push_binding g x t) g (push_binding (mk_env g.f) x t)
+
+let extends_with_push (g1 g2 g3:env)
+  (x:var { ~ (Set.mem x (dom g1)) }) (t:typ)
+  : Lemma (requires extends_with g1 g2 g3)
+          (ensures extends_with (push_binding g1 x t) g2 (push_binding g3 x t)) =
+  assert (equal (push_binding g1 x t)
+                (push_env g2 (push_binding g3 x t)))
+
+let push_context g ctx r = { g with ctxt = Pulse.RuntimeUtils.extend_context ctx (Some r) g.ctxt }
+let push_context_no_range g ctx = { g with ctxt = Pulse.RuntimeUtils.extend_context ctx None g.ctxt }
+
+let get_context g = g.ctxt
+
+let range_of_env (g:env) = 
+    let ctx = T.unseal g.ctxt in
+    match FStar.List.Tot.tryFind (fun (_, r) -> Some? r) ctx with
+    | Some (_, Some r) -> r
+    | _ -> FStar.Range.range_0
+  
+
+
+let ctxt_elt_to_string (c : (string & option range)) : T.Tac string = 
+  match snd c with
+  | None -> fst c
+  | Some r -> Printf.sprintf ("%s @ %s") (fst c) (T.range_to_string r)
+
+let ctx_to_string (c:list (string & option range)) : T.Tac string =
+    match c with
+    | [] -> ""
+    | _ -> 
+      Printf.sprintf "\n\tContext:\n\t%s" (String.concat "\n\t" (T.map ctxt_elt_to_string c))
+
+let ctxt_to_list (g:env) : T.Tac (list string) =
+  let ctx = T.unseal g.ctxt in
+  T.map ctxt_elt_to_string ctx
+
+let print_context (g:env) : T.Tac string = 
+  let ctx = T.unseal g.ctxt in
+  match ctx with
+  | [] -> ""
+  | _ -> 
+    Printf.sprintf "\n\tContext:\n\t%s" (String.concat "\n\t" (ctxt_to_list g))
+
+let print_issue (g:env) (i:FStar.Issue.issue) : T.Tac string = 
+    let open FStar.Issue in
+    let range_opt_to_string = function
+      | None -> "Unknown range"
+      | Some r -> T.range_to_string r
+    in
+    Printf.sprintf "%s (%s): %s%s"
+       (range_opt_to_string (range_of_issue i))
+       (level_of_issue i)
+       (message_of_issue i)
+       (ctx_to_string (T.unseal (get_context g) @ (T.map (fun i -> (i, None)) (context_of_issue i))))
+
+let print_issues (g:env)
+                 (i:list FStar.Issue.issue)
+   = String.concat "\n" (T.map (print_issue g) i)
+
+let fail (#a:Type) (g:env) (r:option range) (msg:string) =
+  let r = 
+    match r with
+    | None -> range_of_env g
+    | Some r -> r
+  in
+  let issue = FStar.Issue.mk_issue "Error" msg (Some r) None (ctxt_to_list g) in
+  FStar.Tactics.log_issues [issue];
+  T.fail "Pulse checker failed"
