pulse/lib/steel/pulse/Pulse.Prover.Substs.fsti
@@ -1,0 +1,126 @@
+module Pulse.Prover.Substs
+
+open FStar.List.Tot
+
+open Pulse.Syntax
+open Pulse.Typing.Env
+
+module L = FStar.List.Tot
+
+module RT = FStar.Reflection.Typing
+module T = FStar.Tactics
+
+module Env = Pulse.Typing.Env
+
+val t (g:env) : Type0
+
+val as_subst (#g:env) (s:t g) : subst
+
+val as_map (#g:env) (s:t g) : Map.t var term
+
+let relates_to (g:env) (s:subst) (m:Map.t var term) =
+  (forall (elt:subst_elt).{:pattern L.memP elt s}
+          L.memP elt s ==> (NT? elt /\
+                            (let NT x t = elt in
+                             Map.contains m x /\
+                             Map.sel m x == t))) /\
+  
+  (forall (x:var).{:pattern Map.contains m x}
+                  Map.contains m x ==> (L.memP (NT x (Map.sel m x)) s)) /\
+
+  (forall (x:var).{:pattern Map.contains m x}
+                  Map.contains m x ==> ((~ (Set.mem x (dom g))) /\
+                                        freevars (Map.sel m x) `Set.subset` dom g))
+
+val subst_as_map (#g:env) (s:t g)
+  : Lemma (relates_to g (as_subst s) (as_map s))
+          [SMTPat (as_subst s); SMTPat (as_map s)]
+
+let dom (#g:_) (s:t g) : Set.set var = Map.domain (as_map s)
+
+let lookup (#g:_) (s:t g) (x:var { x `Set.mem` dom s }) : term =
+  Map.sel (as_map s) x
+
+let equal (#g:env) (s1 s2:t g) =
+  Set.equal (dom s1) (dom s2) /\
+  (forall (x:var).{:pattern Set.mem x (dom s1)} Set.mem x (dom s1) ==> lookup s1 x == lookup s2 x)
+
+val equal_elim (#g:_) (s1 s2:t g)
+  : Lemma (requires equal s1 s2)
+          (ensures s1 == s2)
+          [SMTPat (equal s1 s2)]
+
+val empty (g:env) : t g
+
+val empty_dom (g:_)
+  : Lemma (dom (empty g) == Set.empty)
+          [SMTPat (dom (empty g))]
+
+val singleton (g:env)
+  (x:var { ~ (Set.mem x (Env.dom g)) })
+  (e:term { freevars e `Set.subset` Env.dom g })
+  : t g
+
+val singleton_dom (#g:_)
+  (x:var { ~ (Set.mem x (Env.dom g)) })
+  (e:term { freevars e `Set.subset` Env.dom g })
+  : Lemma (ensures dom (singleton g x e) == Set.singleton x)
+          [SMTPat (dom (singleton g x e))]
+
+val push (#g:_) (s1:t g) (s2:t g { Set.disjoint (dom s1) (dom s2)})
+  : t g
+
+val push_substs_as_map (#g:_) (s1 s2:t g)
+  : Lemma (requires Set.disjoint (dom s1) (dom s2))
+          (ensures as_map (push s1 s2) == Map.concat (as_map s1) (as_map s2))
+          [SMTPat (as_map (push s1 s2))]
+
+let subst_extends (#g:_) (s1 s2:t g) =
+  exists s3. s1 == push s2 s3
+
+let subst_term (#g:_) (s:t g) (t:term) =
+  subst_term t (as_subst s)
+
+let subst_st_term (#g:_) (s:t g) (t:st_term) =
+  subst_st_term t (as_subst s)
+
+let subst_comp (#g:_) (s:t g) (c:comp) =
+  subst_comp c (as_subst s)
+
+val push_subst_term (#g:_) (s1 s2:t g) (t:term)
+  : Lemma (requires Set.disjoint (dom s1) (dom s2))
+          (ensures subst_term (push s1 s2) t ==
+                   subst_term s2 (subst_term s1 t))
+          [SMTPat (subst_term s2 (subst_term s1 t))]
+
+val push_subst_st_term (#g:_) (s1 s2:t g) (t:st_term)
+  : Lemma (requires Set.disjoint (dom s1) (dom s2))
+          (ensures subst_st_term (push s1 s2) t ==
+                   subst_st_term s2 (subst_st_term s1 t))
+          [SMTPat (subst_st_term s2 (subst_st_term s1 t))]
+
+val push_subst_comp (#g:_) (s1 s2:t g) (c:comp)
+  : Lemma (requires Set.disjoint (dom s1) (dom s2))
+          (ensures subst_comp (push s1 s2) c ==
+                   subst_comp s2 (subst_comp s1 c))
+          [SMTPat (subst_comp s2 (subst_comp s1 c))]
+
+val subst_closed_term (#g:_) (s:t g) (t:term)
+  : Lemma (requires freevars t `Set.subset` Env.dom g)
+          (ensures subst_term s t == t)
+
+val subst_closed_st_term (#g:_) (s:t g) (t:st_term)
+  : Lemma (requires freevars_st t `Set.subset` Env.dom g)
+          (ensures subst_st_term s t == t)
+
+val subst_closed_comp (#g:_) (s:t g) (c:comp)
+  : Lemma (requires freevars_comp c `Set.subset` Env.dom g)
+          (ensures subst_comp s c == c)
+
+val diff (#g:_) (s1:t g) (s2:t g { Set.subset (dom s2) (dom s1) })
+  : s3:t g { Set.disjoint (dom s3) (dom s2) }
+
+val diff_push (#g:_) (s1 s2:t g)
+  : Lemma (requires Set.subset (dom s2) (dom s1))
+          (ensures push (diff s1 s2) s2 == s1)
+          [SMTPat (diff s1 s2)]
